\title{Formulas}
\author{Barry Wittman}


\documentclass[12pt]{article}


\usepackage{amsmath}

%\usepackage{kmath}
%\usepackage[math]{anttor}
%\usepackage{millennial}
%\usepackage{fouriernc}
%\usepackage[varg]{txfonts}
\usepackage[charter]{mathdesign}
%\usepackage{fourier}

\usepackage{noto}
\usepackage[T1]{fontenc}

\begin{document}

$$
M = P \cdot \frac{J}{1 - (1 + J)^{-N}}
$$

$$
\frac{-b \pm \sqrt{b^2 - 4ac}}{2a}
$$



$$
\begin{bmatrix}
1 & 0 & 0 \\
0 & \cos \theta & -\sin \theta \\
0 & \sin \theta  & \cos \theta \\
\end{bmatrix}
$$

$$
v'_i = \sum_{j = 1}^n A_{ij}\cdot v_j
$$

$$
\sigma = \sqrt{\frac{1}{n - 1}\sum_{i = 1}^n (x_i - \mu)^2}
$$

$$
f(x) = \sqrt{x}
$$

$$
F = \frac{Gm_1m_2}{r^2}
$$

$$
d = \sqrt{(x_1 - x_2)^2 + (y_1 - y_2)^2 + (z_1 -  z_2)^2}
$$

$$
d = \sqrt{(x_1 - x_2)^2+(y_1 - y_2)^2}
$$

$$
\mathbf{F}_{ab} = - G \frac{m_a m_b}{{\vert \mathbf{r}_{ab} \vert}^2} \, \mathbf{\hat{r}}_{ab}
$$

$$
\mathbf{\hat{r}}_{ab} = \frac{\mathbf{r}_b - \mathbf{r}_a}{\vert\mathbf{r}_b - \mathbf{r}_a\vert}
$$



\end{document}